SkipList2/SkipList.Remove.fst
@@ -1,0 +1,29 @@
+module SkipList.Remove
+
+
+(* last element is less than the next one*)
+val _change_values: #a: eqtype -> #f: cmp a -> s1: seq a {Seq.sorted f s /\ element = Seq.index_last} ->  s: seq a {Seq.sorted f s }-> index: nat {index > place /\ index < Seq.length s} -> 
+Tot (r: seq a {Seq.sorted f s }) 
+let _change_values #a #f s index = 
+	assert (f (Seq.index last ) (Seq.index s index)  );
+	let s1 = append_right s1 (Seq.index s index);
+	assert (Seq.sorted f s1)
+
+val change_values: #a: eqtype -> #f: cmp a -> s: seq a {Seq.sorted  f s } -> Tot(r: seq a {Seq.sorted f r})
+let change_values #a #f s = 
+	_change_values #a #f s place
+	
+	
+
+val _change_indexes_seq: #a: eqtype -> #f : cmp a -> s: seq a -> counter_global : nat {counter_global < Seq.length s} -> 
+	Tot(r: seq a {Seq.length s = Seq.length r + 1})
+
+let _change_indexes_seq : #a: eqtype -> #f: cmp a -> s: seq a -> counter_local : nat {counter_local < List.length (getIndex s counter_global)} -> 
+	let 
+
+val change_indexes: #a: eqtype -> #f : cmp a -> s: seq a -> Tot(r: seq a {Seq.length s = Seq.length r + 1})
+let change_indexes #a #f s = 
+		
+
+val change: #a: eqtype -> #f: cmp a -> sl: skipList a f {Sl.length sl > 1} -> Tot(r: skipList a f {Sl.length sl= Sl.length r + 1 })
+let change 
