SkipList2/SkipList2.Search.fst
@@ -2,6 +2,7 @@ module SkipList2.Search
 
 open SkipList2.Statement
 open SkipList2.Properties
+open SkipList2.Insertion2
 open FStar.Option
 open FStar.Seq
 open FStar.List.Tot
@@ -17,134 +18,111 @@ val prevElement: #a: eqtype -> #f: cmp a -> sl: skipList a f {Sl.length sl > 1}-
 val prevIndex: #a: eqtype -> #f : cmp a -> sl:  skipList a f{Sl.length sl > 1} -> index : nat -> Tot(option(a))
 
 val search: #a: eqtype -> #f: cmp a -> sl: skipList a f {Sl.length sl > 1}-> element : a -> 
-        Tot(option(place: nat { place < Sl.length sl /\ element = getValue sl place}))        
+		Tot(option(place: nat { place < Sl.length sl /\ element = getValue sl place}))		
 
 val exist: #a: eqtype -> #f: cmp a -> sl: skipList a f{Sl.length sl >1} -> element : a -> Tot(bool)
 
-val split: #a: eqtype -> #f : cmp a -> sl: skipList a f -> element : a -> Tot(skipList a f)
-
 type searchResult (a:eqtype) (f:cmp a) (sl: skipList a f) (value: a) (counter_global_previous: nat) = 
 | NotFound: 
-    counter_global : nat 
-        {
-        counter_global > counter_global_previous /\
-        counter_global < (Sl.length sl -1) /\ 
-        (f (getValue sl counter_global) value)
-        }
-    -> searchResult a f sl value counter_global_previous
+	counter_global : nat 
+		{
+		counter_global > counter_global_previous /\
+		counter_global < (Sl.length sl -1) /\ 
+		(f (getValue sl counter_global) value)
+		}
+	-> searchResult a f sl value counter_global_previous
 | Found:  
-    option(
-        place: nat
-            { 
-                place < Sl.length sl /\ value = getValue sl place
-            }
-    )
-     -> searchResult a f sl value counter_global_previous
+	option(
+		place: nat
+			{ 
+				place < Sl.length sl /\ value = getValue sl place
+			}
+	)
+	 -> searchResult a f sl value counter_global_previous
 
 private val searchPlaceIndex: #a: eqtype -> #f : cmp a -> 
-    sl: skipList a f {Sl.length sl > 1} -> 
-    value : a -> 
-    counter_global: nat {counter_global < Sl.length sl } -> 
-    counter_local : nat {counter_local < List.length (getIndex sl counter_global)}-> 
-    Tot(searchResult a f sl value counter_global)
+	sl: skipList a f {Sl.length sl > 1} -> 
+	value : a -> 
+	counter_global: nat {counter_global < Sl.length sl } -> 
+	counter_local : nat {counter_local < List.length (getIndex sl counter_global)}-> 
+	Tot(searchResult a f sl value counter_global)
 
 let rec searchPlaceIndex #a #f sl value counter_global counter_local = 
-    let values = getValues sl in 
-    let index = lemma_index_1_2_wrapper #a #f sl counter_global counter_local in 
-    lemma_last_element_biggest #a #f sl value;
-    if (value = Seq.index values index) then Found (Some index)
-    else if (f (Seq.index values index) value) then 
-        NotFound index
-    else if ((f value (Seq.index values index)) && (counter_local > (List.length (getIndex sl counter_global) -1))) 
-        then searchPlaceIndex #a #f sl value counter_global (counter_local+1)
-    else Found(None)
+	let values = getValues sl in 
+	let index = lemma_index_1_2_wrapper #a #f sl counter_global counter_local in 
+	lemma_last_element_biggest #a #f sl value;
+	if (value = Seq.index values index) then Found (Some index)
+	else if (f (Seq.index values index) value) then 
+		NotFound index
+	else if ((f value (Seq.index values index)) && (counter_local > (List.length (getIndex sl counter_global) -1))) 
+		then searchPlaceIndex #a #f sl value counter_global (counter_local+1)
+	else Found(None)
 
 private val searchPlaceSequence: #a: eqtype ->  #f : cmp a ->  
-                        sl: skipList a f {Sl.length sl > 1} ->  
-                        value : a -> counter_global:nat {counter_global < (Sl.length sl)}->
-                        Tot(option(place: nat { place < Sl.length sl /\ value = getValue sl place}))
-                        (decreases(Sl.length sl- counter_global))
+						sl: skipList a f {Sl.length sl > 1} ->  
+						value : a -> counter_global:nat {counter_global < (Sl.length sl)}->
+						Tot(option(place: nat { place < Sl.length sl /\ value = getValue sl place}))
+						(decreases(Sl.length sl- counter_global))
 
 let rec searchPlaceSequence #a #f sl value counter_global = 
-    let result = searchPlaceIndex #a #f sl value counter_global 0 in 
-    match result with 
-        | Found a -> a 
-        | NotFound counter_global_new -> searchPlaceSequence #a #f sl value counter_global_new        
+	let result = searchPlaceIndex #a #f sl value counter_global 0 in 
+	match result with 
+		| Found a -> a 
+		| NotFound counter_global_new -> searchPlaceSequence #a #f sl value counter_global_new		
 
 private val searchPlace: #a : eqtype -> #f: cmp(a) -> sl: skipList a f {Sl.length sl > 1} -> value : a -> 
-            Tot(option(place: nat { place < Sl.length sl /\ value = getValue sl place}))
+			Tot(option(place: nat { place < Sl.length sl /\ value = getValue sl place}))
 
 let searchPlace #a #f sl value =
-    let counter_global = 0 in 
-    if (value = (Seq.index(getValues sl) counter_global)) then 
-        Some counter_global 
-    else if (Sl.length sl = 1) then None
-    else 
-        searchPlaceSequence #a #f sl value counter_global    
+	let counter_global = 0 in 
+	if (value = (Seq.index(getValues sl) counter_global)) then 
+		Some counter_global 
+	else if (Sl.length sl = 1) then None
+	else 
+		searchPlaceSequence #a #f sl value counter_global	
 
 let search #a #f sl element = 
-    searchPlace #a #f sl element
+	searchPlace #a #f sl element
 
 let nextElement #a #f sl element = 
-    let place = searchPlace #a #f sl element in 
-    match place with
-        | None -> None 
-        | Some place -> 
-            if ((place +1) < Sl.length sl) then 
-                Some(getValue sl (place+1))
-            else None    
+	let place = searchPlace #a #f sl element in 
+	match place with
+		| None -> None 
+		| Some place -> 
+			if ((place +1) < Sl.length sl) then 
+				Some(getValue sl (place+1))
+			else None	
 let nextIndex #a #f sl index = 
-    if (index + 1 < Sl.length sl) then 
-        Some (getValue sl (index+1))
-    else None            
+	if (index + 1 < Sl.length sl) then 
+		Some (getValue sl (index+1))
+	else None			
 
 let prevElement #a #f sl element = 
-    let place = searchPlace #a #f sl element in 
-    match place with 
-        | None -> None
-        | Some place -> 
-            if (place -1) > 0 then 
-                Some (getValue sl (place-1))
-            else None    
+	let place = searchPlace #a #f sl element in 
+	match place with 
+		| None -> None
+		| Some place -> 
+			if (place -1) > 0 then 
+				Some (getValue sl (place-1))
+			else None	
 
 let prevIndex #a #f sl index = 
-    if (index -1 > 0 && (index-1) < Sl.length sl) then 
-        Some (getValue sl (index -1)) 
-    else None    
+	if (index -1 > 0 && (index-1) < Sl.length sl) then 
+		Some (getValue sl (index -1)) 
+	else None	
 
 let exist #a #f sl element = 
-    let r = search #a #f sl element in 
-    match r with 
-    | None -> false
-    | Some _ -> true
+	let r = search #a #f sl element in 
+	match r with 
+	| None -> false
+	| Some _ -> true
 
 val _forall: listFrom : list nat -> predicate: (nat -> Tot bool) -> pred_yes: (nat -> Tot nat) -> pred_no : (nat -> Tot nat) -> 
-            Tot(r: list nat{List.length listFrom = List.length r})
+			Tot(r: list nat{List.length listFrom = List.length r})
 
 let rec _forall listFrom predicate pred_yes pred_no = 
-    match listFrom with 
-    | [] -> []
-    | a::tl -> let elem = if predicate a then pred_yes a 
-                else pred_no a in elem :: 
-                _forall tl predicate pred_yes pred_no 
-
-val _list_tr : listFrom : list nat-> compare: nat ->change : nat  -> 
-        Tot(listTo: list nat{List.length listFrom = List.length listTo})
-
-let _list_tr listFrom compare change = 
-    let predicate = (fun x -> x < compare) in 
-    let predicate_yes = (fun x -> x) in 
-    let predicate_no = (fun x -> change) in 
-    _forall listFrom predicate predicate_yes predicate_no
-
-val seqRegeneration:sFrom: seq (list nat){Seq.length sFrom > 0}  -> i: nat {i <= Seq.length sFrom} -> 
-                    compare: nat ->change : nat ->  
-                    Tot(r: seq (list nat) {Seq.length sFrom = Seq.length r})(decreases(Seq.length sFrom - i))
-
-(* *abstract val upd: #a:Type -> s:seq a -> n:nat{n < length s} -> a ->  Tot (seq a) (decreases (length s))*)
-let rec seqRegeneration sFrom i compare change =
-    if (i < Seq.length sFrom) then 
-        let elem = _list_tr (Seq.index sFrom i) compare change in 
-        let s = Seq.upd sFrom i elem in seqRegeneration s (i+1) compare change
-    else 
-        sFrom   
+	match listFrom with 
+	| [] -> []
+	| a::tl -> let elem = if predicate a then pred_yes a 
+				else pred_no a in elem :: 
+				_forall tl predicate pred_yes pred_no 
