SkipList2/SkipList2.Seq.Properties.fst
@@ -1,0 +1,153 @@
+module SkipList2.Seq.Properties
+
+open FStar.Seq
+open FStar.Option
+
+module Seq = FStar.Seq
+module List = FStar.List.Tot
+
+type cmp (a:eqtype) = f:(a -> a -> Tot bool){total_order a f}
+
+val seqLast: s: seq 'a {Seq.length s > 0}-> Tot 'a
+let seqLast s = 
+	(Seq.index s (Seq.length s -1))
+
+val tail_mem : 	#a : eqtype -> #f: cmp a -> 
+			pivot : a -> 
+			s : seq a {Seq.sorted f s /\ Seq.length s > 0 /\ Seq.mem pivot  s = false /\ f (seqLast s) pivot } ->
+			Lemma (ensures (forall y. (Seq.mem y s ==> f y pivot)))(decreases (Seq.length s))
+
+let rec tail_mem #a #f pivot s = 
+	if (Seq.length s = 1) then () else
+	tail_mem #a #f pivot (Seq.tail s)	
+
+val tail_mem_wrapper: #a : eqtype -> 
+			#f: cmp a -> 
+			pivot : a -> 
+			s : seq a {Seq.sorted f s /\ Seq.length s > 0 /\ 
+					Seq.mem pivot  s = false /\ f (seqLast s) pivot } -> 
+			Tot(r: seq a {(forall y. (Seq.mem y r ==> f y pivot))})
+
+let tail_mem_wrapper #a #f pivot s = 
+	tail_mem #a #f pivot s; s		
+
+val right_tail_mem: #a: eqtype -> #f: cmp a -> pivot : a -> s: seq a { Seq.sorted f s /\ Seq.length s > 0 /\ Seq.mem pivot s = false /\ 
+			f pivot (Seq.index s 0)} -> 
+			Lemma (ensures (forall y. (Seq.mem y s ==> f pivot y)))(decreases (Seq.length s))
+
+let rec right_tail_mem #a #f pivot s = 
+	if (Seq.length s = 1) then () else
+	right_tail_mem #a #f pivot (Seq.tail s)	
+
+val right_tail_mem_wrapper: #a: eqtype -> #f: cmp a -> pivot : a -> 
+			s: seq a { Seq.sorted f s /\ Seq.length s > 0 /\ Seq.mem pivot s = false /\ 
+			f pivot (Seq.index s 0)} -> 
+			Tot(r: seq a {(forall y. (Seq.mem y r ==> f pivot y))})	
+
+let right_tail_mem_wrapper #a #f pivot s = right_tail_mem #a #f pivot s; s	
+
+assume val temp_lemma_split: #a : eqtype -> #f: cmp a -> pivot : a -> s: seq a 
+								{Seq.sorted f s /\ Seq.length s > 0 /\ 
+								Seq.mem pivot  s = false} ->
+								place : nat {place < Seq.length s} -> 
+								Lemma (ensures 
+									( 
+										(Seq.sorted f (fst(Seq.split s place))) /\ 
+										(Seq.length (fst(Seq.split s place)) > 0) /\
+										(Seq.mem pivot (fst(Seq.split s place)) = false) /\
+										(Seq.sorted f (snd(Seq.split s place))) /\ 
+										(Seq.length (snd(Seq.split s place)) > 0) /\
+										(Seq.mem pivot (snd(Seq.split s place)) = false) 
+								))
+
+val temp_lemma_split_wrapper: #a : eqtype -> #f: cmp a -> pivot : a -> 
+								s: seq a 
+									{Seq.sorted f s /\ Seq.length s > 0 /\ 
+									Seq.mem pivot  s = false} ->
+								place : nat {place < Seq.length s  } ->  
+								Tot(r: seq a
+								{
+									(Seq.sorted f r)/\ 
+									(Seq.length r > 0) /\
+									(Seq.mem pivot r = false) /\ Seq.length r = place
+								})
+
+let temp_lemma_split_wrapper #a #f pivot s place =
+	let r = fst(Seq.split s place) in 
+		temp_lemma_split #a #f pivot s place; r
+
+val temp_lemma_split_wrapper_right: #a : eqtype -> #f: cmp a -> pivot : a -> 
+								s: seq a 
+									{Seq.sorted f s /\ Seq.length s > 0 /\ 
+									Seq.mem pivot  s = false} ->
+								place : nat {place < Seq.length s  } ->  
+								Tot(r: seq a
+								{
+									(Seq.sorted f r)/\ 
+									(Seq.length r > 0) /\
+									(Seq.mem pivot r = false) /\ Seq.length r = (Seq.length s) - place
+								})
+
+let temp_lemma_split_wrapper_right #a #f pivot s place =
+	let r = snd(Seq.split s place) in temp_lemma_split #a #f pivot s place; r
+
+val tail_mem_split: #a : eqtype -> 
+					#f: cmp a -> 
+					pivot : a ->
+					s: seq a{Seq.sorted f s /\ Seq.length s > 0 /\ Seq.mem pivot s = false } -> 
+					place : nat{place < Seq.length	s -1 /\ f (Seq.index s place) pivot} -> 
+					Tot(r: seq a {(forall y. (Seq.mem y r ==> f y pivot))})
+
+let tail_mem_split #a #f pivot s place = 
+	let seq_new = temp_lemma_split_wrapper #a #f pivot s (place+1)  in 
+	tail_mem_wrapper #a #f pivot seq_new
+
+val right_tail_mem_split : #a : eqtype -> 
+					#f: cmp a -> 
+					pivot : a ->
+					s: seq a{Seq.sorted f s /\ Seq.length s > 0 /\ Seq.mem pivot s = false } -> 
+					place : nat{place < Seq.length s  /\ f pivot (Seq.index s (place))} -> 
+					Tot(r: seq a {(forall y. (Seq.mem y r ==> f pivot y ))})
+
+let right_tail_mem_split #a #f pivot s place = 
+	let seq_new = temp_lemma_split_wrapper_right #a #f pivot s (place)  in 
+	right_tail_mem_wrapper #a #f pivot seq_new
+
+val main_lemma_split: #a : eqtype -> 
+					#f: cmp a -> 
+					pivot : a ->
+					s: seq a{Seq. sorted f s /\ Seq.length s > 0 /\ Seq.mem pivot s = false } ->
+					place : nat{place  < Seq.length s -1  /\ f (Seq.index s place) pivot /\ f pivot (Seq.index s (place+1))} -> 
+					Tot(r1: seq a {(forall y. (Seq.mem y r1 ==> f y pivot))} * r2: seq a {(forall y. (Seq.mem y r2 ==> f pivot y ))})
+
+let main_lemma_split #a #f pivot s place =
+	(tail_mem_split #a #f pivot s (place), right_tail_mem_split #a #f pivot s (place+1))
+
+val split_0 : #a: eqtype -> s: seq a{Seq.length s > 0} -> Lemma(
+															ensures(
+																Seq.equal (snd(Seq.split s 0)) s))
+let split_0 #a s = ()
+
+val sorted_seq_concat_wrapper : #a: eqtype -> #f: cmp a ->pivot : a -> s1: seq a 
+			{Seq.sorted f s1 /\ (forall y. (Seq.mem y s1 ==> f y pivot))} ->  
+			s2: seq a {Seq.sorted f s2 /\ (forall y. (Seq.mem y s2 ==> f pivot y))}  ->
+		  	Tot(s3: seq a{Seq.sorted f s3 /\ Seq.length s3 = Seq.length s1 + Seq.length s2 + 1}) 
+
+let sorted_seq_concat_wrapper #a #f pivot s1 s2 = 
+		let s3 = (Seq.append s1 (cons pivot s2)) in 
+		FStar.Seq.Properties.sorted_concat_lemma #a f s1 pivot s2; 
+		s3  
+(*pivot is not used*)
+val ordered_addition_0: 
+	#a: eqtype -> #f: cmp a -> pivot: a -> s2: seq a {Seq.sorted f s2 /\ (forall y. (Seq.mem y s2 ==> f pivot y))} ->
+				Tot(s3: seq a{Seq.sorted f s3 /\ Seq.length s3 = Seq.length s2 + 1}) 
+
+let ordered_addition_0 #a #f pivot s2 = 
+		let s1 = Seq.createEmpty in 
+		sorted_seq_concat_wrapper #a #f pivot s1 s2 	
+
+val upd: l: list 'a -> counter: nat -> value: 'a -> Tot(r: list 'a{List.length l = List.length r})
+let rec upd l counter value = 
+	match l with
+	| hd::tl -> if (counter = 0) then value:: tl else hd::upd tl (counter-1) value
+	| [] -> []		
